\documentclass[12pt]{article}
\usepackage{fullpage,enumitem,amsmath,amssymb,graphicx}

\begin{document}

\begin{center}
{\Large CS221 Fall 2013 Homework: Images}

\begin{tabular}{rl}
SUNet ID: & nisham \\
Name: & Nisha Masharani \\
Collaborators: & sryoung, alesan92
\end{tabular}
\end{center}

By turning in this assignment, I agree by the Stanford honor code and declare
that all of this is my own work.

\section*{Problem 1}

\begin{enumerate}[label=(\alph*)]
  \item To minimize $\sum_{i=1}^{n} \|x_i-\mu_{z_i}\|_2^2$, take the derivative with respect to $\mu_k$ and set it to zero. In this case, because we are taking the derivative of the sum, all elements of the sum where $\mu_{z_i} \ne \mu_k$ go to zero, and we are left with a sum over all elements where $z_i = k$.

  \begin{eqnarray*}
  \frac{d}{d\mu_k}\biggl[\sum_{i=1}^{n} \|x_i-\mu_{z_i}\|_2^2\biggr] &=& \sum_{i:z_i = k} \|x_i-\mu_{z_i}\|_2 \\
  \end{eqnarray*}

  We then set the derivative to be zero, and solve for $\mu_k$. We can pull $\mu_k$ out of the sum because it is a constant.

  \begin{eqnarray*}
  \sum_{i:z_i = k} \|x_i-\mu_{z_i}\|_2 &=& 0\\
  \sum_{i:z_i = k} \|x_i-\mu_k\|_2 &=& 0\\
  -\mu_k * |{i:z_i = k}| + \sum_{i:z_i = k} \|x_i\| &=& 0\\
  \sum_{i:z_i = k} \|x_i\| &=& \mu_k * |{i:z_i = k}|\\

  \end{eqnarray*}

  \item (your solution)
\end{enumerate}

\section*{Problem 2}

\begin{enumerate}[label=(\alph*)]
  \item (your solution)
  \item (your solution)
\end{enumerate}

\end{document}
